Update client proof in demo_cpp_proof

rocq-brick-libstdcpp/proof/mutex/demo_cpp_proof.v
@@ -9,8 +9,10 @@ Require Import bluerock.brick.libstdcpp.mutex.demo_cpp.
 Proof. solve_learnable. Qed.
 
 Definition TT : tele := [tele (_ : Z) (_ : Z)].
-Definition mk (a b : Z) : TT :=
+
+Polymorphic Definition mk (a b : Z) : TT :=
   {| tele_arg_head := a; tele_arg_tail := {| tele_arg_head := b; tele_arg_tail := () |} |}.
+Succeed Definition b := recursive_mutex.Held 0 (mk 0 0).
 
 br.lock
 Definition P `{Σ : cpp_logic, σ : genv} (this : ptr) : TT -t> mpred :=
@@ -21,13 +23,14 @@ Definition P `{Σ : cpp_logic, σ : genv} (this : ptr) : TT -t> mpred :=
 br.lock
 Definition CR
     `{Σ : cpp_logic, σ : genv, HasOwn mpredI recursive_mutex.cmraR}
-    (γ : gname) (q : cQp.t) : Rep :=
+    (γ : recursive_mutex.rmutex_gname) (q : cQp.t) : Rep :=
   structR "C" q **
-  _field "C::mut" |-> recursive_mutex.R γ q **
+  _field "C::mut" |-> recursive_mutex.R γ.(recursive_mutex.lock_gname) q **
   as_Rep (fun this : ptr =>
     recursive_mutex.inv_rmutex γ (∃ a_b : tele_arg _, tele_app (P this) a_b)).
 
-#[only(type_ptr, lazy_unfold)] derive CR.
+#[only(cfractional,ascfractional,type_ptr)] derive CR.
+#[only(lazy_unfold)] derive CR.
 
 Section with_cpp.
   Context `{Σ : cpp_logic}.
@@ -35,46 +38,81 @@ Section with_cpp.
   Context {HAS_THREADS : HasStdThreads Σ}.
   Context {has_rmutex : HasOwn mpredI recursive_mutex.cmraR}.
 
-  cpp.spec "C::update_a(int)" with
+  cpp.spec "C::update_a(int)" as C_update_a with
     (\this this
      \arg{x} "x" (Vint x)
      \prepost{γ q} this |-> CR γ q
-     \prepost{q'} recursive_mutex.token γ q'
+     \prepost{q'} recursive_mutex.token γ.(recursive_mutex.lock_gname) q'
      \pre{args th} recursive_mutex.acquireable γ th args (TT:=TT) (P this)
      \post recursive_mutex.acquireable γ th (TT:=TT) (recursive_mutex.update (TT:=TT) (fun (a b : Z) => mk (a+x) b) args) (P this)).
 
-  cpp.spec "C::update_b(int)" with
+  cpp.spec "C::update_b(int)" as C_update_b with
     (\this this
      \arg{x} "x" (Vint x)
      \prepost{γ q} this |-> CR γ q
-     \prepost{q'} recursive_mutex.token γ q'
+     \prepost{q'} recursive_mutex.token γ.(recursive_mutex.lock_gname) q'
      \pre{args th} recursive_mutex.acquireable γ th args (TT:=TT) (P this)
      \post recursive_mutex.acquireable γ th (TT:=TT) (recursive_mutex.update (TT:=TT) (fun (a b : Z) => mk a (b + x)) args) (P this)).
+
+  #[global] Instance CR_learn : Cbn (Learn (learn_eq ==> any ==> learn_hints.fin) CR).
+  Proof. solve_learnable. Qed.
+
+  Import recursive_mutex.
+
+  #[program]
+  Definition acquireable_acquireable_C γ :=
+    \cancelx
+    \consuming{th n args P} acquireable (TT := TT) γ th (Held n args) P
+    \bound P'
+    \bound_existential th' args'
+    \proving acquireable γ th' args' P'
+    \instantiate th' := th
+    \instantiate args' := Held n args
+    \deduce tele_app P args
+    \through tele_app P' args
+    \end.
+  Next Obligation. rewrite acquireable.unlock; work. Qed.
+
+  Hint Resolve acquireable_acquireable_C : br_hints.
+
+  #[program]
+  Definition own_P_is_acquireable_C' γ n :=
+    \cancelx
+    \preserving{th} current_thread th
+    \consuming own γ.(level_gname) (◯E (S n, th))
+    \bound (P : TT -t> mpred)
+    \bound_existential th'
+    \bound_existential st
+    \proving acquireable (TT := TT) γ th' st P
+    \instantiate th' := th
+    \bound a b
+    \instantiate st := Held n (mk a b)
+    \through tele_app P (mk a b)
+    \end.
+  Next Obligation. rewrite acquireable.unlock; work. Qed.
+  (* XXX this hint isn't robust because [a] and [b] become evars bound. *)
+
 
   Lemma update_a_ok : verify[source] "C::update_a(int)".
   Proof.
     verify_spec; go.
-    work.
+    iExists _, TT, (P this), _, th.
+    go.
 
-    iExists TT; iExists (P this). iExists th.
-    go.
     rewrite P.unlock /=.
-    (* Instance token_learn γ : LearnEq1 (recursive_mutex.token γ) := ltac:(solve_learnable). *)
     destruct args as [a [b []]]; simpl; go.
-    iSplitR. { admit. (* TODO make the addition modulo arithmetic in the spec *) }
+    wfocus [| valid<_> _|] "". {
+      admit. (* TODO make the addition modulo arithmetic in the spec *)
+    }
     go.
-    iExists TT; iExists (P this).
-    iExists th.
+    iExists _, TT, (P this).
+    rewrite P.unlock.
+    iExists _, th.
     iExists n, (mk (a + x) b).
-    rewrite P.unlock. go.
-    (* Clients shouldn't unfold abstractions like [recursive_mutex.acquireable] *)
-    rewrite /recursive_mutex.acquireable.
-    work.
-    erewrite recursive_mutex.update_eq; last done.
     go.
     rewrite P.unlock. go.
-    (* Clients shouldn't do case distinctions! *)
-    destruct n; rewrite /recursive_mutex.acquireable; go.
+    erewrite recursive_mutex.update_eq; last done.
+    work.
     all: fail.
   Admitted.
 
@@ -82,30 +120,39 @@ Section with_cpp.
     (\this this
       \arg{x} "x" (Vint x)
       \prepost{γ q} this |-> CR γ q
-      \prepost{q'} recursive_mutex.token γ q'
+      \prepost{q'} recursive_mutex.token γ.(recursive_mutex.lock_gname) q'
       \pre{args th} recursive_mutex.acquireable γ th args (TT:=TT) (P this)
       \post recursive_mutex.acquireable γ th (TT:=TT) (recursive_mutex.update (TT:=TT) (fun (a b : Z) => mk (a+x) (b-x)) args) (P this)).
 
   Lemma transfer_ok : verify[source] "C::transfer(int)".
   Proof.
     verify_spec; go.
-    rewrite /CR. go.
-    iExists TT; iExists (P this). iExists th. iExists _. go.
-    iExists _; iExists th. go.
-    iExists _; iExists th. go.
-    cut_pure (valid<"int"> _).
-    { admit. (* TODO make the addition modulo arithmetic in the spec *) }
+    iExists γ, TT, (P this), _, th.
     go.
-    iExists TT; iExists (P this); iExists th; iExists _.
+    iExists γ.
+    rewrite !P.unlock /=.
     work.
-    iFrame.
-    rewrite /CR. work.
-    destruct n; subst; simpl; work.
-    destruct args as [a[b?]]; simpl.
-    have->: (b + (0 - x) = b - x)%Z by lia. done.
+    destruct args as [a[b []]]; simpl.
+    work.
+
+    Set Warnings "-br-hint-leading-to-dangling-evars".
+    go using own_P_is_acquireable_C'.
+    Set Warnings "br-hint-leading-to-dangling-evars".
+
+    wfocus [| valid<_> _|] "". {
+      admit. (* TODO make the addition modulo arithmetic in the spec *)
+    }
+
+    rewrite !P.unlock /=.
+    go.
+    iExists _, TT, (P this), _, th.
+    rewrite !P.unlock /=.
+    work.
+    erewrite recursive_mutex.update_eq; last done.
+    rewrite !P.unlock /=.
+    work.
     all: fail.
   Admitted.
 
 End with_cpp.
 
-Import auto_frac auto_pick_frac.
